\documentclass[11pt]{article}
\usepackage[margin = 1in]{geometry}
\usepackage{amsmath}
\usepackage{amssymb}
\usepackage{amsthm} % for proof environment
\usepackage{enumitem}
\usepackage{graphicx}
\usepackage{indentfirst}
\usepackage{caption}
\usepackage{lscape}
\usepackage{multirow}
\usepackage{array}

\renewcommand{\labelenumii}{\alph*)}
\newcommand{\w}{\omega}
\newcommand{\p}{\prime}
\newcommand{\one}{\mathbf{1}}
\newcommand{\lagr}{\mathcal{L}}
\newcommand{\inv}[1]{#1^{-1}}
\newcommand{\ev}{\mathbb{E}}

\begin{document}
	
\begin{flushleft}
	Nick Hoffman \\
	Finance I, Spring 2020 A \\
	Assignment 1 \\
\end{flushleft}

\begin{enumerate}
	\item Useful facts
	\begin{enumerate}
		\item $ \ev[\w ^\p R ] = \w^\p \bar{R} $, where $\bar{R}$ is the $ N\times 1 $ vector of expected returns.
		\[\ev[\w^\p \bar{R}] = \ev\left[\sum_{i = 1}^{N}\tilde{R}_n \w_n\right] = \sum_{i = 1}^N \w_n \ev[\tilde{R}_n] = \w^\p \bar{R} \]
		
		\item 
	\end{enumerate}
	\item 
	\item 
	\item 
	\begin{gather*}
	\min_\w \frac{1}{2}\w^\p V \w \\
	\text{s.t.} \\
	(1 - \w^\p \one)R_f + \w^\p \bar{R} \geq \mu
	\end{gather*}
	\begin{enumerate}
		\item Wish to show that the solution to this problem can be written as 
		\[\w = \gamma \w^*\]
		where 
		\begin{gather*}
			\w^{*\p}\one = 1\text{, and} \\
			\w^* = \alpha \w_R + (1 - \alpha)\w_1
		\end{gather*}
		with 
		\begin{align*}
		\w_R &= \frac{\inv{V}\bar{R}}{\one^\p \inv{V} \bar{R}} \\
		\w_1 &= \frac{\inv{V} \one}{\one^\p \inv{V} \one}
		\end{align*}
		The Lagrangian for this problem is as follows:
		\[\lagr = \frac{1}{2}\w^\p V \w + \lambda \big[\mu - (1 - \w^\p \one)R_f - \w^\p \bar{R}\big] \]
		with first-order conditions
		\begin{align}
		V\w + \lambda(\one R_f - \bar{R}) &= \mu \label{foc_4_1}\\
		(1 - \w^\p \one)R_f + \w^\p \bar{R} &\geq \mu \label{foc_4_2}
		\end{align}
		To begin, premultiply (\ref{foc_4_1}) by $ \inv{V} $ (assuming that $ V $ is invertible):
		\[\w = \lambda \inv{V} \bar{R} - \lambda \inv{V} \one R_f\]
		We can solve for $ \w $ as a function of $ \w_R $ and $ \w_1 $ as before:
		\begin{align*}
		\w &= \lambda \left[\left(\frac{\one^\p \inv{V} \bar{R}}{\one^\p \inv{V} \bar{R}}\right)\inv{V}\bar{R} - \left(\frac{\one^\p \inv{V} \one}{\one^\p \inv{V} \one}\right)\inv{V}\one^\p R_f\right] \\
		&= \lambda \big[(\one^\p \inv{V}\bar{R})\w_R - (\one^\p \inv{V}\one R_f)\w_1\big]
		\end{align*}
		
	\end{enumerate}
\end{enumerate}

\end{document}